Deep type checking
Bug fixes:

- Fix variable binding time (in `wp_decl_var`).
  Variables become available before they are initialized.
  This bug would have allowed us to verify a program like:
  ```
  int x = 0;
  { int x = x; }
  ```
  The second line should have UB because the `x` on the RHS refers
  to the declaration on line 2, not the one on line 1.

- Fix typing of globals `Eglobal`, adding `tref`

- Fix printer for decomposition decls (`Ddecompose`)

Also,

- Improve the shallow type checker
- Rework casts
- Improve members, member pointers, subscripts
- Hoist parsec, some traversals, and an error type

include/CoqPrinter.hpp
@@ -68,12 +68,14 @@ public:
 		return this->output_ << fmt::tuple_sep;
 	}
 
-	fmt::Formatter& ctor(llvm::StringRef ctor, bool line = true) {
+	template<typename T>
+	fmt::Formatter& ctor(T ctor, bool line = true) {
 		if (line) {
 			this->output_ << fmt::line;
 		}
 		return this->output_ << fmt::lparen << ctor << fmt::nbsp;
 	}
+
 	fmt::Formatter& end_ctor() {
 		return this->output_ << fmt::rparen;
 	}
