theories/lang/cpp/syntax/typed.v
@@ -1,0 +1,858 @@
+(*
+ * Copyright (c) 2023-2024 BedRock Systems, Inc.
+ * This software is distributed under the terms of the BedRock Open-Source License.
+ * See the LICENSE-BedRock file in the repository root for details.
+ *)
+
+Require Import bedrock.lang.cpp.syntax.prelude.
+Require Import bedrock.lang.cpp.syntax.core.
+Require Import bedrock.lang.cpp.syntax.types.
+Require Import bedrock.lang.cpp.syntax.typing.
+Require Import bedrock.lang.cpp.syntax.stmt.
+Require Import bedrock.lang.cpp.syntax.namemap.
+Require Import bedrock.lang.cpp.syntax.translation_unit.
+Import UPoly.
+
+#[local] Open Scope monad_scope.
+
+(* TODO: a little "sloppy" with the errors *)
+mlock Definition breadcrumb {t : Set} (_ : t) : Error.t := inhabitant.
+mlock Definition Bad_allocation_function_args {lang : lang.t} (_ : list (type' lang)) : Error.t := inhabitant.
+mlock Definition Can_initialize {lang : lang.t} (dt it : decltype' lang) : Error.t := inhabitant.
+
+Module decltype.
+
+  (**
+  [to_exprtype] decomposes a declaration type into a value category
+  and expression type. This is delicate because xvalue references to
+  function types induce lvalue expressions.
+
+  [to_valcat] is similar, but keeps only the value category. Matching
+  on [to_valcat t] is simpler than matching on [t] when [t] might be
+  an xvalue reference to a function type.
+  *)
+  Definition to_exprtype {lang} (t : decltype' lang) : ValCat * exprtype' lang :=
+    match drop_qualifiers t with
+    | Tref u => (Lvalue, u)
+    | Trv_ref u =>
+      match drop_qualifiers u with
+      | Tfunction _ as f =>
+        (**
+        Both "a function call or an overloaded operator expression,
+        whose return type is rvalue reference to function" and "a cast
+        expression to rvalue reference to function type" are lvalue
+        expressions.
+
+        This also applies to <<__builtin_va_arg>> (an extension).
+
+        https://en.cppreference.com/w/cpp/language/value_category#lvalue
+        https://www.eel.is/c++draft/expr.call#13
+        https://www.eel.is/c++draft/expr.static.cast#1
+        https://www.eel.is/c++draft/expr.reinterpret.cast#1
+        https://www.eel.is/c++draft/expr.cast#1 (C-style casts)
+
+        NOTE: We return the function type without qualifiers in light
+        of "A function or reference type is always cv-unqualified."
+        <https://www.eel.is/c++draft/basic.type.qualifier#1>
+        *)
+        (Lvalue, f)
+      | _ => (Xvalue, u)
+      end
+    | _ => (Prvalue, t)	(** Promote sharing, rather than normalize qualifiers *)
+    end.
+  Definition to_valcat {lang} (t : decltype' lang) : ValCat := (to_exprtype t).1.
+
+  (**
+  Compute a declaration type from a value category and expression
+  type.
+
+  Up to dropping qualifiers on reference and function types, this is
+  intended to be a partial inverse of [to_exprtype].
+  *)
+  Definition of_exprtype {lang} (vc : ValCat) (t : exprtype' lang) : decltype' lang :=
+    (**
+    As [t : Mexprtype], we do not need [tref], [trv_ref].
+    *)
+    match vc with
+    | Lvalue => Tref t
+    | Xvalue => Trv_ref t
+    | Prvalue => t
+    end.
+
+  Module internal.
+  Section with_lang.
+    Context {lang : lang.t}.
+    #[local] Notation Expr := (Expr' lang).
+    #[local] Notation decltype := (decltype' lang).
+    #[local] Notation exprtype := (exprtype' lang).
+    #[local] Notation function_type := (function_type' lang).
+    #[local] Notation functype := (functype' lang).
+    #[local] Notation Stmt := (Stmt' lang).
+
+    #[local] Definition M : Set -> Set := (readerT.M (decltype * option exprtype * list (localname * decltype)) (trace.M Error.t)).
+    #[local] Instance M_Ret : MRet M := _.
+    #[local] Instance M_Ap : Ap M := _.
+    #[local] Instance M_Bind : MBind M := _.
+    #[local] Instance M_Fail : MFail M := _.
+    #[local] Instance M_Throw : Trace Error.t M := _.
+    #[local] Hint Opaque M : typeclass_instances.
+
+    Definition ask_return : M decltype :=
+      readerT.asks (fun '(a,_,_) => a).
+    Definition ask_this : M exprtype :=
+      let* rt := readerT.asks (fun '(_,this,_) => this) in
+      match rt with
+      | None => mfail
+      | Some ty => mret ty
+      end.
+    Definition of_option {T : Set} (o : option T) : M T :=
+      match o with
+      | None => mfail
+      | Some v => mret v
+      end.
+
+    (* Bindings *)
+    Record bindings : Set := { _bindings : list (localname * decltype) }.
+    Instance bindings_empty : Empty bindings := {| _bindings := nil |}.
+    Definition with_var {T} (x : localname) (t : decltype) : M T -> M T :=
+      readerT.local (fun '(ret, this, vars) => (ret, this, (x,t) :: vars)).
+    Definition with_bindings {T} (b : bindings) (m : M T) : M T :=
+      fold_right (fun xt => with_var xt.1 xt.2) m b.(_bindings).
+    #[local] Instance bindings_monoid : monoid.Monoid bindings :=
+      {| monoid.monoid_unit := bindings_empty
+       ; monoid.monoid_op a b := {| _bindings := a.(_bindings) ++ b.(_bindings) |} |}.
+
+    Definition var_type (n : localname) : M decltype :=
+      let* vars := readerT.asks (fun '(_,_,vars) => vars) in
+      match List.find (fun x => bool_decide (x.1 = n)) vars with
+      | None => trace (breadcrumb ("failed to find variable "%bs, n, " in "%bs, vars)) $ mfail
+      | Some t => mret t.2
+      end.
+
+    (**
+    The declaration type of an explicit cast to type [t] or a call to
+    a function or overloaded operator returning type [t] or a
+    [__builtin_va_arg] of type [t].
+    *)
+    Definition normalize (t : decltype) : decltype :=
+      let p := to_exprtype t in
+      of_exprtype p.1 p.2.
+
+    (** Function return type *)
+    Definition from_function_type (ft : function_type) : decltype :=
+      normalize ft.(ft_return).
+    Definition from_functype (t : functype) : M decltype :=
+      match t with
+      | Tfunction ft => mret $ from_function_type ft
+      | _ => mfail
+      end.
+    Definition require_functype (t : decltype) : M function_type :=
+      match t with
+      | Tfunction ft => mret ft
+      | _ => mfail
+      end.
+    Definition require_mfunctype (t : decltype) : M (decltype * function_type) :=
+      match t with
+      | Tmember_pointer nm ft => pair nm <$> require_functype ft
+      | _ => mfail
+      end.
+
+    Section fixpoint.
+      Context (of_expr : Expr -> M decltype).
+      Context (of_stmt : Stmt -> M (option decltype)).
+
+      Definition of_unop (op : UnOp) (t : exprtype) : M decltype :=
+        match op with
+        | Uminus | Uplus =>
+          if is_arithmetic t then mret t else mfail (* TODO: check this *)
+        | Unot => if is_arithmetic t then mret Tbool else mfail
+        | Ubnot => if is_arithmetic t then mret t else mfail
+        | Uunsupported _ => mfail
+        end.
+
+      Definition of_binop (op : BinOp) (l r : decltype) (t : exprtype) : M decltype :=
+        match op with
+        | Bdotp =>
+          (**
+          The value category of [e1.*e2] is (i) that of [e1] (xvalue
+          or lvalue) when [e2] points to a field and (ii) prvalue when
+          [e2] points to a method.
+
+          We need only address (i) here because when [e2] is a method,
+          the result of [e1.*e2] must be immediately applied, and
+          cpp2v emits [Emember_call] rather than [Ebinop] for indirect
+          method calls.
+
+          https://www.eel.is/c++draft/expr.mptr.oper#6
+          *)
+          match l with
+          | Trv_ref _ => mret $ Trv_ref t
+          | _ => mret $ Tref t
+          end
+        | Bdotip => mret $ Tref t	(* derived from [Bdotp] *)
+        | _ => mret t
+        end.
+
+      Definition of_member (Et : bool * exprtype) (mut : bool) (t : decltype) : M decltype :=
+        let '(ref, et) := to_exprtype t in
+        match ref with
+        | Lvalue | Xvalue => mret $ Tref et
+        | Prvalue =>
+          let oty := Et.2 in
+          let qual :=
+            let '(ocv, _) := decompose_type oty in
+            CV (if mut then false else q_const ocv) (q_volatile ocv)
+          in
+          let ty := tqualified qual et in
+          if Et.1 then mret $ Trv_ref ty else mret $ Tref ty
+        end.
+
+      Definition of_subscript (t1 t2 : decltype) (t : exprtype) : M decltype :=
+        (* we need to handle arrays and pointers.
+           Arrays can be lvalues or xvalues.
+         *)
+        match drop_qualifiers t1 , drop_qualifiers t2 with
+        | Tref aty , Tnum _ _ => tref QM <$> of_option (array_type aty)
+        | Trv_ref aty , Tnum _ _ => trv_ref QM <$> of_option (array_type aty)
+        | Tptr ety , Tnum _ _ => mret $ Tref ety
+        | Tnum _ _ , Tref aty => tref QM <$> of_option (array_type aty)
+        | Tnum _ _ , Trv_ref aty => trv_ref QM <$> of_option (array_type aty)
+        | Tnum _ _ , Tptr ety => mret $ Tref ety
+        | _ , _ => mfail
+        end.
+
+      Definition requireL (t : decltype) : M exprtype :=
+        match t with
+        | Tref t => mret t
+        | _ => mfail
+        end.
+      Definition requireGL_get (t : decltype) : M (bool * exprtype) :=
+        match t with
+        | Tref t => mret (false, t)
+        | Trv_ref t => mret (true, t)
+        | _ => mfail
+        end.
+      Definition requireGL (t : decltype) : M exprtype :=
+        match t with
+        | Tref t | Trv_ref t => mret t
+        | _ => mfail
+        end.
+      Definition requirePR (t : decltype) : M exprtype :=
+        match t with
+        | Tref _ | Trv_ref _ => mfail
+        | _ => mret t
+        end.
+      Definition requireR (t : decltype) : M exprtype :=
+        match t with
+        | Tref _ => mfail
+        | _ => mret t
+        end.
+      Definition require_eq {T : Set} {_ : EqDecision T} (l : T) (r : T) : M unit :=
+        trace (breadcrumb ("require equal "%bs, l, " = "%bs, r)) $
+        const () <$> guard (l = r).
+
+      (* determine if this type can be used in an <<if>> *)
+      Definition require_testable (t : exprtype) : M unit :=
+        match t with
+        | Tnum _ _
+        | Tptr _
+        | Tbool
+        | Tnullptr
+        | Tchar_ _
+        | Tfloat_ _ => mret ()
+        | _ => mfail
+        end.
+
+      Definition require_ptr (t : decltype) : M exprtype :=
+        match t with
+        | Tptr t => mret t
+        | _ => mfail
+        end.
+
+      Definition arrow_deref (arrow : bool) : decltype -> M exprtype :=
+        if arrow then require_ptr else requireGL.
+      Definition arrow_deref_get (arrow : bool) : decltype -> M (bool * exprtype) :=
+        if arrow then fun t => pair false <$> require_ptr t else requireGL_get.
+
+
+      Notation "a >=> b" := (a >>= b) (at level 61, left associativity).
+
+      Definition can_initialize (dt : decltype) (t : decltype) : M unit :=
+        trace (Can_initialize dt t) $
+          let* _ := guard (drop_qualifiers dt = drop_qualifiers t) in
+          mret ().
+
+      Fixpoint check_args (ar : function_arity) (ts : list decltype) (tes : list decltype) : M unit :=
+        match ts , tes with
+        | nil , nil => mret ()
+        | t :: ts , te :: tes =>
+            (* toplevel qualifiers on arguments are ignored *)
+            let* _ := can_initialize t te in
+            check_args ar ts tes
+        | nil , te :: tes =>
+            match ar with
+            | Ar_Variadic => mret () (* TODO: should check that all arguments can be passed as variadic arguments *)
+            | _ => mfail
+            end
+        | _ , _ => mfail
+        end.
+
+      Definition of_cast (c : Cast_ (type' lang) (type' lang)) (base : decltype) : M decltype :=
+        match c with
+        | Cdependent t
+        | Cbitcast t
+        | Clvaluebitcast t => mret t
+        | Cl2r dt =>
+            let* et := requireGL base in
+            let* _ := requirePR dt >>= require_eq (drop_qualifiers et) in
+            mret dt
+        | Cnoop t => mret t
+        | Carray2ptr t =>
+            let k cv base :=
+              match base with
+              | Tarray ty _
+              | Tincomplete_array ty
+              | Tvariable_array ty _ =>
+                  let res := Tptr $ tqualified cv ty in
+                  let* _ := require_eq t res in
+                  mret res
+              | _ => mfail
+              end
+            in
+            requireGL base >>= qual_norm k
+        | Cfun2ptr t =>
+            let* base := requireL base in
+            let* _ := require_functype base in
+            let* _ := require_eq t (Tptr base) in
+            mret $ Tptr base
+        | Cint2ptr t
+        | Cptr2int t => mret t
+        | Cptr2bool => mret Tbool
+        | Cderived2base [] _
+        | Cbase2derived [] _ => mfail (* empty lists are not supported *)
+        | Cderived2base (l :: ls) t => mret t (* TODO *)
+        | Cbase2derived (l :: ls) t => mret t (* TODO *)
+
+        | Cintegral t => mret t
+        | Cint2bool => mret Tbool
+        | Cfloat2int t
+        | Cnull2ptr t
+        | Cnull2memberptr t
+        | Cbuiltin2fun t
+        | Cctor t => mret t
+        | C2void => mret Tvoid
+        | Cuser => mret base
+        | Cdynamic to => mret to
+        end.
+
+      Definition of_expr_body (e : Expr) : M decltype :=
+        trace (breadcrumb e) $
+        let* result :=
+        match e return M decltype with
+        | Eparam X => mret $ Tresult_param X
+        | Eunresolved_global on => mret $ Tresult_global on
+        | Eunresolved_unop o e => Tresult_unop o <$> of_expr e
+        | Eunresolved_binop o l r => Tresult_binop o <$> of_expr l <*> of_expr r
+        | Eunresolved_call on es => Tresult_call on <$> traverse (T:=eta list) of_expr es
+        | Eunresolved_member_call on obj es => Tresult_member_call on <$> of_expr obj <*> traverse (T:=eta list) of_expr es
+        | Eunresolved_parenlist (Some t) es => Tresult_parenlist t <$> traverse (T:=eta list) of_expr es
+        | Eunresolved_parenlist None _ => mfail
+        | Eunresolved_member obj fld => Tresult_member <$> of_expr obj <*> mret fld
+
+        | Evar ln t =>
+            let* vt := var_type ln in
+            let* _ := require_eq t vt in
+            mret $ tref QM t
+        | Eenum_const n _ => mret $ Tenum n
+        | Eglobal nm ty => mret $ tref QM ty
+        | Eglobal_member nm ty =>
+            match nm with
+            | Nscoped cls _ =>
+              mret $ Tmember_pointer (Tnamed cls) ty
+            | _ => mfail
+            end
+
+        | Echar _ t =>
+            match t with
+            | Tchar_ _
+            | Tuchar | Tschar => mret t
+            | _ => mfail
+            end
+        | Estring chars t =>
+            mret $ Tref $ Tarray (Qconst t) (1 + list_numbers.lengthN chars)
+        | Eint _ t =>
+            let* _ := guard (t ∈ [Tchar;Tuchar;Tschar;Tshort;Tushort;Tint;Tuint;Tlong;Tulong;Tlonglong;Tulonglong]) in
+            mret t
+        | Ebool _ => mret Tbool
+        | Eunop op e t =>
+            let* et := of_expr e >>= requirePR in
+            let* t' := of_unop op et >>= requirePR in
+            let* _ := guard (t = t') in
+            mret t
+        | Ebinop op l r t =>
+            let* lt := of_expr l in
+            let* rt := of_expr r in
+            of_binop op lt rt t
+        | Ederef e t =>
+            let* t' := of_expr e >>= require_ptr in
+            let* _ := guard (t = t') in
+            mret $ Tref t
+        | Eaddrof e =>
+            let* t := of_expr e >>= requireGL in
+            mret $ Tptr t
+        | Eassign le re t =>
+            let* lt := of_expr le >>= requireL in
+            let* rt := of_expr re >>= requireR in
+            let* _ := guard (lt = rt) in
+            let* _ := guard (lt = t) in
+            mret $ Tref lt
+        | Eassign_op op le re t =>
+            (* TODO: i still need to check that the operation is permitted at this type *)
+            let* lt := of_expr le >>= requireL in
+            let* rt := of_expr re >>= requireR in
+            let* _ := guard (lt = t) in
+            mret $ Tref lt
+        | Epreinc e t
+        | Epredec e t =>
+            (* TODO: <<+>>or <<->> must be valid *)
+            let* lt := of_expr e >>= requireL in
+            let* _ := guard (lt = t) in
+            mret $ Tref lt
+        | Epostinc e t
+        | Epostdec e t =>
+            (* TODO: <<+>>or <<->> must be valid *)
+            let* lt := of_expr e >>= requireL in
+            let* _ := guard (lt = t) in
+            mret lt
+
+        | Eseqand le re
+        | Eseqor le re =>
+            let* _ := of_expr le >>= require_testable in
+            let* _ := of_expr re >>= require_testable in
+            mret Tbool
+        | Ecomma e1 e2 =>
+            let* _ := of_expr e1 in
+            of_expr e2
+        | Ecall f es =>
+            let* ft := of_expr f >=> require_ptr >=> require_functype in
+            let* ts := traverse (T:=eta list) of_expr es in
+            let* _ := check_args ft.(ft_arity) ft.(ft_params) ts in
+            mret ft.(ft_return)
+        | Eexplicit_cast _ t e =>
+            let cast_result :=
+              qual_norm (fun cv t =>
+                           match t with
+                           | Tnamed _
+                           | Tarray _ _
+                           | Tincomplete_array _
+                           | Tvariable_array _ _
+                           | Tenum _ => tqualified cv t
+                           | _ => t
+                           end)
+            in
+            let* ct := of_expr e in
+            let* _ := require_eq ct (cast_result t) in
+            (* ^^ in the case of pr-values, type qualifiers do not need to match *)
+            mret $ cast_result t
+            (*   ^ we return [t] to match the shallow checker, but we would
+                 probably prefer dropping qualifiers *)
+        | Ecast c e => of_expr e >>= of_cast c
+        | Emember arrow e _ mut t =>
+            let* edt := of_expr e >>= arrow_deref_get arrow in
+            of_member edt mut t
+        | Emember_call arrow f obj es =>
+            let* objT := of_expr obj >>= arrow_deref arrow in
+            let* tes := traverse (T:=eta list) of_expr es in
+            let* ft :=
+              match f with
+              | inl (_, _, ft) => require_functype ft
+              | inr e =>
+                  let* ft := of_expr e in
+                  match ft with
+                  | Tmember_pointer cls (Tfunction ft) =>
+                      mret ft
+                  | _ => mfail
+                  end
+              end
+            in
+            let* _ := check_args ft.(ft_arity) ft.(ft_params) tes in
+            mret ft.(ft_return)
+
+        | Eoperator_call _ f es =>
+            let* tes := traverse (T:=eta list) of_expr es in
+            let* '(result, fargs) :=
+              match f with
+              | operator_impl.Func _ ft =>
+                  let* ft := require_functype ft in
+                  mret (ft.(ft_return), ft.(ft_params))
+              | operator_impl.MFunc _ _ ft =>
+                  (* TODO: the type of the member function does not currently
+                     contain the [Tmember_pointer] type *)
+                  let* objT :=
+                    match tes with
+                    | obj :: _ => mret [obj]
+                    | _ => mret []
+                    end
+                  in
+                  let* ft := require_functype ft in
+                  mret (ft.(ft_return), objT ++ ft.(ft_params))
+              end
+            in
+            let* _ := check_args Ar_Definite fargs tes in
+            mret result
+        | Esubscript e1 e2 t =>
+            let* t1 := of_expr e1 in
+            let* t2 := of_expr e2 in
+            of_subscript t1 t2 t
+        | Esizeof te t
+        | Ealignof te t =>
+            let* _ :=
+              match te with
+              | inl t => mret ()
+              | inr e => const () <$> of_expr e
+              end
+            in
+            const Tsize_t <$> guard (t = Tsize_t)
+        | Eoffsetof _ _ t => mret t
+        | Econstructor f es t =>
+            (* TODO: check the type of the constructor [f] *)
+            let* tes := traverse (T:=eta list) of_expr es in
+            mret t
+        | Eimplicit e => of_expr e
+        | Eimplicit_init t =>
+            (**
+          "References cannot be value-initialized".
+
+          https://en.cppreference.com/w/cpp/language/value_initialization
+             *)
+
+            let* _ := requirePR t in
+            mret t
+        | Eif tst thn els t =>
+            let* _ := of_expr tst >>= require_testable in
+            let* tthn := of_expr thn >>= require_eq t in
+            let* tels := of_expr els >>= require_eq t in
+            mret t
+        | Eif2 x lete tst thn els t =>
+            let* lt := of_expr lete in
+            with_var (localname.anon x) lt $
+              let* _ := of_expr tst >>= require_testable in
+              let* tthn := of_expr thn in
+              let* _ := of_expr els >>= require_eq tthn in
+              let* _ := guard (t = tthn) in
+              mret t
+        | Ethis t =>
+            let* pt := require_ptr t in
+            let* _ := ask_this >>= require_eq pt in
+            mret t
+        | Enull => mret Tnullptr
+        | Einitlist es oe t =>
+            let* _ := traverse (T:=eta list) of_expr es in
+            let* _ :=
+              match oe with
+              | None => mret tt
+              | Some e => const tt <$> of_expr e
+              end
+            in
+            mret t
+        | Enew (alloc, alloc_ty) aes nf aty osz oinit =>
+            let* ats := traverse (T:=eta list) of_expr aes in
+            let* afty := require_functype alloc_ty in
+            let* _ :=
+              let* _ := guard (afty.(ft_return) = Tptr Tvoid) in
+              let* params :=
+                match afty.(ft_params) return M (list decltype) with
+                | Tsize_t :: params => mret params
+                | args => trace (Bad_allocation_function_args args) $ mfail
+                end
+              in
+              let* params :=
+                if nf is new_form.Allocating true then
+                  match params with
+                  | Talign_t :: params => mret params
+                  | _ => trace (Bad_allocation_function_args afty.(ft_params)) mfail
+                  end
+                else
+                  mret params
+              in
+              check_args afty.(ft_arity) params ats
+            in
+            let* _ :=
+              match osz with
+              | None => mret tt
+              | Some sz =>
+                  let* tsz := of_expr sz in
+                  if is_arithmetic tsz then mret tt else mfail
+              end
+            in
+            let* _ :=
+              match oinit with
+              | None => mret tt
+              | Some init => let* _ := of_expr init in mret tt (* TODO: check result type against [aty] *)
+              end
+            in
+            mret $ Tptr aty
+        | Edelete _ (del, del_ty) e ty =>
+            let* et := of_expr e >>= require_ptr in
+            let* _ := guard (ty = et) in (* TODO: constness check? *)
+            mret Tvoid
+        | Eandclean e => of_expr e
+        | Ematerialize_temp e vc =>
+            let* _ := guard (vc <> Prvalue) in
+            of_exprtype vc <$> (of_expr e >>= requirePR)
+        | Eatomic _ es t =>
+            let* tes := traverse (T:=eta list) of_expr es in
+            mret t
+        | Estmt s t =>
+            let* st := of_stmt s in
+            let* _ := require_eq st (Some t) in
+            mret t
+        | Eva_arg e t =>
+            let* _ := of_expr e in (* TODO: what type should this have? *)
+            mret $ normalize t
+        | Epseudo_destructor arr t e =>
+            let* et := of_expr e >>= arrow_deref arr in
+            let* _ := require_eq t (drop_qualifiers et) in
+            mret Tvoid
+        | Earrayloop_init n e level _ e2 t =>
+            let* _ := of_expr e in
+            let* _ :=
+              with_var (localname.arrayloop_index level) Tsize_t $
+                       with_var (localname.opaque n) t $
+                of_expr e2 in
+            mret t
+        | Earrayloop_index n t =>
+            let* _ := var_type (localname.arrayloop_index n) >>= require_eq t in
+            mret t (* always pr-values? *)
+        | Eopaque_ref n t =>
+            let* vt := var_type (localname.opaque n) in
+            let* _ := requireGL t >>= can_initialize vt in
+            (* ^^ in practice, the type and the recorded variable type
+               differ by <<const>> qualifiers in instance-specific ways *)
+            mret t
+        | Eunsupported _ t => mret t
+        end
+        in
+        let* _ :=
+          let shallow := decltype_of_expr e in
+          trace (breadcrumb ("type mismatch"%bs, result, shallow)) $ require_eq result shallow
+        in
+        mret result.
+    End fixpoint.
+
+    Definition big_op `{Mon : monoid.Monoid m} `{Traverse T} (ls : T m) : m :=
+      writer.value $ traverse (F:=writer.M m) (T:=T) (writer.tell) ls.
+
+    Section var_decl.
+      Context (of_expr : Expr -> M decltype).
+
+      Fixpoint check_decl (d : VarDecl' lang) : M bindings :=
+        trace (breadcrumb d)
+        match d with
+        | Dvar lname ty oinit =>
+            let* _ :=
+              match oinit with
+              | None => mret tt
+              | Some init =>
+                  let* _ := with_var lname ty $ of_expr init >>= can_initialize ty in
+                  mret tt
+              end
+            in
+            mret ({| _bindings := [(lname, ty)] |})
+        | Ddecompose e v ds =>
+            (* TODO: this is wrong, it requires a more subtle binding form because [e] is bound during the
+              evaluation of the declarations, but is unbound afterwards *)
+            let* t := of_expr e in
+            let* (bindings : list bindings) := with_var v t $ traverse (T:=eta list) check_decl ds in
+            mret $ big_op bindings
+        | Dinit _ nm ty oinit =>
+            let* _ :=
+              match oinit with
+              | None => mret tt
+              | Some init =>
+                  let* _ := of_expr init >>= can_initialize ty in
+                  mret tt
+              end
+            in
+            mret monoid.monoid_unit
+        end.
+
+    End var_decl.
+
+    Section stmt.
+      Context (of_expr : Expr -> M decltype).
+
+      Notation check_decl := (check_decl of_expr) (only parsing).
+
+      Definition check_decls (ds : list (VarDecl' lang)) : M bindings :=
+        big_op (T:=eta list) <$> traverse (F:=M) (T:=eta list) check_decl ds.
+
+      Fixpoint check_stmt_body (s : Stmt' lang) : M (bindings * option decltype) :=
+        let check_stmt := check_stmt_body in
+        trace (breadcrumb s)
+        match s with
+        | Sgoto _ => mret (∅, None)
+        | Slabeled _ s => check_stmt s
+        | Sexpr e =>
+            pair monoid.monoid_unit ∘ Some <$> of_expr e
+        | Sdefault | Scase _ | Sbreak | Scontinue => mret (∅, None)
+        | Sseq ss =>
+            (fix block ss :=
+               match ss with
+               | nil => mret (∅, None)
+               | s :: ss =>
+                   let* '(b,d) := check_stmt s in
+                   with_bindings b $ block ss
+               end) ss
+        | Sif vd tst thn els =>
+            let* ds := from_option check_decl (mret monoid.monoid_unit) vd in
+            let* _ :=
+              with_bindings ds $
+                let* _ := of_expr tst >>= require_testable in
+                let* _ := check_stmt thn in
+                check_stmt els
+            in mret (∅, None)
+        | Sswitch vd tst b =>
+            let* ds := from_option check_decl (mret monoid.monoid_unit) vd in
+            let _ :=
+              with_bindings ds $
+                let* _ := of_expr tst >>= require_eq Tint in (* TODO: BAD *)
+                check_stmt b
+            in mret (∅, None)
+        | Swhile vd tst body =>
+            let* ds := from_option check_decl (mret monoid.monoid_unit) vd in
+            let k :=
+              with_bindings ds $
+                let* _ := of_expr tst >>= require_testable in
+                check_stmt body
+            in mret (∅, None)
+        | Sdo s tst =>
+            let* _ := check_stmt s in
+            let* _ := of_expr tst >>= require_testable in (* TODO *)
+            mret (∅, None)
+        | Sfor vd otst oincr body =>
+            let* '(ds, _) := from_option check_stmt (mret (monoid.monoid_unit, None)) vd in
+            let* _ :=
+              with_bindings ds $
+                let* _ := from_option (fun e => of_expr e >>= require_testable) (mret tt) $ otst in
+                let* _ := from_option (fun e => let* _ := of_expr e in mret tt) (mret tt) $ oincr in
+                check_stmt body
+            in mret (∅, None)
+        | Sdecl ds =>
+            let* b := check_decls ds in
+            mret (b, None)
+        | Sreturn None =>
+            let* _ := ask_return >>= require_eq Tvoid in
+            mret (∅, None)
+        | Sreturn (Some e) =>
+            let* ret := ask_return in
+            let* _ := of_expr e >>= can_initialize ret in
+            mret (∅, None)
+        | Sattr _ s =>
+            check_stmt s (* TODO: confirm scope *)
+        | Sasm _ _ ins outs args =>
+            let* _ := traverse (T:=eta list) (fun ab => of_expr ab.2) ins in
+            let* _ := traverse (T:=eta list) (fun ab => of_expr ab.2) outs in
+            mret (∅, None)
+        | Sunsupported _ => mfail
+        end.
+    End stmt.
+
+    Fixpoint of_expr (e : Expr) : M decltype :=
+      of_expr_body of_expr check_stmt e
+    with check_stmt (s : Stmt) : M (option decltype) :=
+      snd <$> check_stmt_body of_expr s.
+
+
+    Definition Merr : Set -> Set := trace.M Error.t.
+
+    Definition check_func (f : Func' lang) : Merr unit :=
+      match f.(f_body) with
+      | None => mret ()
+      | Some (Impl body) =>
+          const () <$> readerT.run (with_bindings {| _bindings := f.(f_params) |} $ check_stmt body) (f.(f_return), None, [])
+      | Some (Builtin _) => mret ()
+      end.
+
+    Definition classname_to_type : classname' lang -> type' lang :=
+      match lang with
+      | lang.cpp => Tnamed
+      | lang.temp => id
+      end.
+
+    Definition check_method (m : Method' lang) : Merr unit :=
+      match m.(m_body) with
+      | Some (UserDefined s) =>
+          let this_type := tqualified m.(m_this_qual) $ classname_to_type m.(m_class) in
+          const () <$> readerT.run (with_bindings {| _bindings := m.(m_params) |} $ check_stmt s) (m.(m_return), Some this_type, [])
+      | _ => mret ()
+      end.
+
+    Definition check_ctor (c : Ctor' lang) : Merr unit :=
+      match c.(c_body) with
+      | Some (UserDefined (inits, body)) =>
+          readerT.run (with_bindings {| _bindings := c.(c_params) |} $
+                         let* _ := traverse (T:=eta list) (fun init => of_expr init.(init_init)) inits in
+                         const () <$> check_stmt body) (Tvoid, Some (classname_to_type c.(c_class)), [])
+      | _ => mret ()
+      end.
+
+    Definition check_dtor (d : Dtor' lang) : Merr unit :=
+      match d.(d_body) with
+      | Some (UserDefined body) =>
+          readerT.run (const () <$> check_stmt body) (Tvoid, Some (classname_to_type d.(d_class)), [])
+      | _ => mret ()
+      end.
+
+    Definition check_obj_value (o : ObjValue' lang) : Merr unit :=
+      trace (breadcrumb o)
+      match o with
+      | Ovar _ oinit =>
+          match oinit with
+          | None => mret tt
+          | Some init =>
+              const () <$> readerT.run (of_expr init) (Tvoid, None, []) (* Tvoid isn't really correct here *)
+          end
+      | Ofunction f => check_func f
+      | Omethod m => check_method m
+      | Oconstructor c => check_ctor c
+      | Odestructor d => check_dtor d
+      end.
+
+  End with_lang.
+
+  End internal.
+
+  Definition of_expr {lang} (tu : translation_unit) (e : Expr' lang) : trace.M Error.t (decltype' lang) :=
+    let lookup :=
+      match lang as lang return _ with
+      | lang.cpp => fun nm => fmap (M:=fun t => option t) type_of_value $ tu.(symbols) !! nm
+      | lang.temp => fun _ => None
+      end
+    in
+    readerT.run (internal.of_expr e) (Tvoid, None, []).
+
+  Definition check_tu (tu : translation_unit) : trace.M Error.t unit :=
+    let fn (nm_v : name * ObjValue) :=
+      trace (breadcrumb nm_v.1) $ internal.check_obj_value nm_v.2
+    in
+    let* _ := traverse (T:=eta list) fn $ NM.elements tu.(symbols) in
+    mret tt.
+End decltype.
+
+Module exprtype.
+Section exprtype.
+  Context {lang : lang.t} (tu : translation_unit).
+
+  Definition of_expr (e : Expr' lang) : option (ValCat * exprtype' lang) :=
+    trace.runO $ decltype.to_exprtype <$> decltype.of_expr tu e.
+
+  Definition of_expr_drop (e : Expr' lang) : option (exprtype' lang) :=
+    trace.runO $ drop_reference <$> decltype.of_expr tu e.
+
+  Definition of_expr_check (P : ValCat -> Prop) `{!∀ vc, Decision (P vc)}
+      (e : Expr' lang) : option (exprtype' lang) :=
+    of_expr e >>= fun p => guard (P p.1) ;; mret p.2.
+
+End exprtype.
+End exprtype.
